Adapted PhiInfo to separate out_vars and the function BlockID -> in_sexprs

theories/liveness.v
@@ -75,9 +75,9 @@ Module Liveness (D: DIALECT).
     end.
   
   (* Applies the inverse of the phi function. It is like applying the assignment backwards. *)
-  Definition apply_inv_phi (renamings: InBlockPhiInfo) (s: VarSet.t) :=
+  Definition apply_inv_phi (out_vars: list VarID.t) (renamings: InBlockPhiInfo) (s: VarSet.t) :=
     match renamings with
-    | in_phi_info out_vars in_sexprs => 
+    | in_phi_info in_sexprs => 
         let in_set := list_to_set (extract_yul_vars in_sexprs) in
         let out_set := list_to_set out_vars in
         (VarSet.union (VarSet.diff s out_set) in_set)
@@ -216,7 +216,8 @@ Module Liveness (D: DIALECT).
                     match (f_info next_bid) with
                     | None => false
                     | Some (next_b_in_info,next_b_out_info) =>
-                        VarSet.equal b_out_info (apply_inv_phi (BlockD.phi_function next_b b.(BlockD.bid)) next_b_in_info)
+                     (* VarSet.equal b_out_info (apply_inv_phi (BlockD.phi_function next_b b.(BlockD.bid)) next_b_in_info) *)
+                        VarSet.equal b_out_info (apply_inv_phi (fst next_b.(phi_function)) (snd (next_b.(phi_function)) b.(BlockD.bid)) next_b_in_info)
                     end
                 end
                   
@@ -235,8 +236,10 @@ Module Liveness (D: DIALECT).
                             | None => false
                             | Some (next_b_iff_in_info,next_b_iff_out_info) =>
                                 VarSet.equal b_out_info (VarSet.union
-                                                           (apply_inv_phi (BlockD.phi_function next_b_if_true b.(BlockD.bid)) next_b_ift_in_info)
-                                                           (apply_inv_phi (BlockD.phi_function next_b_if_false b.(BlockD.bid)) next_b_iff_in_info))
+                                (* (apply_inv_phi (BlockD.phi_function next_b_if_true b.(BlockD.bid)) next_b_ift_in_info)
+                                   (apply_inv_phi (BlockD.phi_function next_b_if_false b.(BlockD.bid)) next_b_iff_in_info)) *)
+                                   (apply_inv_phi (fst next_b_if_true.(phi_function)) (snd next_b_if_true.(phi_function) b.(BlockD.bid)) next_b_ift_in_info)
+                                   (apply_inv_phi (fst next_b_if_false.(phi_function)) (snd next_b_if_false.(phi_function) b.(BlockD.bid)) next_b_iff_in_info))
                             end
                         end
                     end
@@ -324,8 +327,7 @@ Module Liveness (D: DIALECT).
                     match (f_info next_bid) with
                     | None => false
                     | Some (next_b_in_info,next_b_out_info) =>
-                        (* VarSet.equal b_out_info (apply_inv_phi (BlockD.phi_function next_b b.(BlockD.bid)) next_b_in_info) *)
-                        VarSet.subset (apply_inv_phi (BlockD.phi_function next_b b.(BlockD.bid)) next_b_in_info) b_out_info
+                        VarSet.subset (apply_inv_phi (fst next_b.(phi_function)) (snd next_b.(phi_function) b.(BlockD.bid)) next_b_in_info) b_out_info
                     end
                 end
                   
@@ -343,12 +345,9 @@ Module Liveness (D: DIALECT).
                             match (f_info next_bid_if_false) with
                             | None => false
                             | Some (next_b_iff_in_info,next_b_iff_out_info) =>
-                               (* VarSet.equal b_out_info (VarSet.union
-                                                           (apply_inv_phi (BlockD.phi_function next_b_if_true b.(BlockD.bid)) next_b_ift_in_info)
-                                                           (apply_inv_phi (BlockD.phi_function next_b_if_false b.(BlockD.bid)) next_b_iff_in_info)) *)
                                 VarSet.subset b_out_info (VarSet.union
-                                                           (apply_inv_phi (BlockD.phi_function next_b_if_true b.(BlockD.bid)) next_b_ift_in_info)
-                                                           (apply_inv_phi (BlockD.phi_function next_b_if_false b.(BlockD.bid)) next_b_iff_in_info))
+                                                           (apply_inv_phi (fst next_b_if_true.(phi_function)) (snd next_b_if_true.(phi_function) b.(BlockD.bid)) next_b_ift_in_info)
+                                                           (apply_inv_phi (fst next_b_if_false.(phi_function)) (snd next_b_if_false.(phi_function) b.(BlockD.bid)) next_b_iff_in_info))
                             end
                         end
                     end
